\section{Problem 1}
\prob{\label{h1:problem1}
    Let $\c{B}$ a combinatoric class withouth $0$-sized elements. Suppose 
		\begin{align}
				\c{M} &= MSet({B})			\\
				\intertext{\center{y}}	\\
				\c{P} &= PSet({B}) 
		\end{align}
		
		Prove that:
		\begin{align}
				M(z) = P(z)M(z^2).
		\end{align}
}

\begin{proof}
We already know that
	\begin{align}
	    M(z) = \prod_{n = 1}^\infty (1 - z^n)^{- B_n}
	\end{align}
	
	and
	\begin{align}
	    P(z) = \prod_{n = 1}^\infty (1 + z^n)^{B_n}.
	\end{align}\pn
	
	Where $B_n$ is the amount of elements in $\c{B}$ of size $n$.\pn	
	
	Then
	\begin{align}
			P(z)M(z^2) 	&=	\paren{\prod_{n = 1}^\infty (1 + z^n)^{B_n}} \cdot \paren{\prod_{n = 1}^\infty (1 - z^{(2n)})^{- B_n}}	\\
									&=	\prod_{n = 1}^\infty (1 + z^n)^{B_n} (1 - z^{(2n)})^{- B_n}																							\\
									&=	\prod_{n = 1}^\infty (1 + z^n)^{B_n} \paren{(1 + z^n)(1 - z^n)}^{- B_n}																	\\
									&=	\prod_{n = 1}^\infty (1 + z^n)^{B_n} (1 + z^n)^{- B_n} (1 - z^n)^{- B_n}																\\
									&=	\prod_{n = 1}^\infty (1 + z^n)^{B_n - B_n} (1 - z^n)^{- B_n}																						\\
									&=	\prod_{n = 1}^\infty (1 - z^n)^{- B_n}																																	\\
									&=	M(z) \qedhere
	\end{align}
\end{proof}