\section{Problem 2}
\prob{\label{h1:problem2}
    Prove that:
    \begin{align}
        \frac{1}{2z} \paren{1 - \sqrt{1 - 4z}} = \sum_{n=0}^\infty \frac{1}{n+1}\binom{2n}{n}z^n
    \end{align}
}

\begin{proof}
    First let remember that if $r \in \R \setminus \Z$, the generalized Newton binomial theorem says that
    
    \begin{align}
            (x + y)^r = \sum_{n = 0}^{\infty} \binom{r}{n} x^{r-n} y^{n}
    \end{align}\pn
    
    Where $\binom{r}{n}$ is defined as
    
    \begin{align}
            \binom{r}{n} = \begin{cases}
                                \frac{r(r-1)\cdots(r-n+1)}{n!} & \text{if } n \geq 1   \\
                                1                              & \text{if } n = 0   \\
                           \end{cases}.
    \end{align}\pn
    
    
    
    With this, we can write $\sqrt{1 - 4z}$ as follows
    
    \begin{align}
            \sqrt{1 - 4z}   &=  \paren{1 - 4z}^{\frac{1}{2}}                                                                                                    \\
                            &=  \sum_{n = 0}^{\infty} \binom{\frac{1}{2}}{n} 1^{\frac{1}{2}-n}(-4z)^{n}                                                         \\
                            &=  \sum_{n = 0}^{\infty} \binom{\frac{1}{2}}{n} (-4z)^{n}                                                                          \\
                            &\intertext{
                                Now, note that the firs term in the sum is $1$, so for convenience we will write this term explicitly}                          \\
                            &=  1 + \sum_{n = 1}^{\infty} \binom{\frac{1}{2}}{n} (-4z)^{n}                                                                          \\
                            &=  1 + \sum_{n = 1}^{\infty} \frac{ \frac{1}{2} (\frac{1}{2}-1) (\frac{1}{2}-2) \cdots (\frac{1}{2}-(n-11)) }{n!} (-4z)^{n}             \\
                            &=  1 + \sum_{n = 1}^{\infty} \frac{ \frac{1}{2} (- \frac{1}{2}) (-\frac{3}{2}) \cdots (-\frac{2n - 3}{2}) }{n!} (-4z)^{n}              \\
                            &=  1 + \sum_{n = 1}^{\infty} (-1)^{n-1} \frac{ \frac{1}{2} (\frac{1}{2}) (\frac{3}{2}) \cdots (\frac{2n - 3}{2}) }{n!} (-4z)^{n}       \\
                            &=  1 + \sum_{n = 1}^{\infty} (-1)^{(2n-1)} \frac{ \frac{1}{2} (\frac{1}{2}) (\frac{3}{2}) \cdots (\frac{2n -3 }{2}) }{n!} (4z)^{n}     \\
                            &=  1 - \sum_{n = 1}^{\infty} \paren{\frac{1}{2^n}} \frac{ 1 \cdot 1 \cdot 3 \cdot 5 \cdots (2n - 3) }{n!} (4z)^{n}                    \\
                            &=  1 - \sum_{n = 1}^{\infty} \paren{\frac{1}{2^n}} \frac{ 1 \cdot 3 \cdot 5 \cdots (2n - 3) }{n!} 2^{2n} (z)^{n}                      \\
                            &=  1 - \sum_{n = 1}^{\infty} \paren{2^n} \frac{ 1 \cdot 3 \cdot 5 \cdots (2n - 3) }{n!} (z)^{n}                                       \\
                            &\intertext{
                                Note that the product in the fraction's numerator is just the product of the first $n-1$ odd numbers, and remember that
                                the product of the first $n-11$ even numbers can be written as $2^{n-1}(n-1)!$. So, given this, we can write the product of the
                                first $n-1$ odd numbers as $\frac{(2n-2)!}{2^{n-1}(n-1)!}$. So, we can now write the previous sum as}
                            &=  1 - \sum_{n = 1}^{\infty} \paren{2^n} \frac{(2n-2)!}{2^{n-1}(n-1)!} \frac{1}{n!} (z)^{n}                                           \\
                            &=  1 - 2 \sum_{n = 1}^{\infty} \frac{(2n-2)!}{(n-1)! n!}  (z)^{n}                                                           \\
                            &=  1 - 2 \sum_{n = 1}^{\infty} \frac{(2n-2)!}{(n-1)! (n-1)! } \frac{1}{n}  (z)^{n}                                                           \\
                            &=  1 - 2 \sum_{n = 1}^{\infty} \binom{2(n-1)}{n-1} \frac{1}{n}  (z)^{n}                                                                 \\
    \end{align}\pn
    
    Now we can rewrite $1 - \sqrt{1 - 4z}$ as
    
    \begin{align}
            1 - \sqrt{1 - 4z}   &=  1 - \paren{1 - 2 \sum_{n = 1}^{\infty} \binom{2(n-1)}{n-1} \frac{1}{n}  (z)^{n}}      \\
                                &=  2 \sum_{n = 1}^{\infty} \binom{2(n-1)}{n-1} \frac{1}{n}  (z)^{n}
    \end{align}\pn
    
    Finally, we can rewrite $\frac{1}{2z} \paren{1 - \sqrt{1 - 4z}}$ as
    
    \begin{align}
            \frac{1}{2z} \paren{1 - \sqrt{1 - 4z}}  &=  \frac{1}{2z} 2 \sum_{n = 1}^{\infty} \binom{2(n-1)}{n-1} \frac{1}{n}  (z)^{n}   \\
                                                    &=  \frac{1}{z} \sum_{n = 1}^{\infty} \binom{2(n-1)}{n-1} \frac{1}{n}  (z)^{n}      \\
                                                    &=  \sum_{n = 1}^{\infty} \binom{2(n-1)}{n-1} \frac{1}{n}  (z)^{n-1}                \\
                                                    &=  \sum_{n = 0}^{\infty} \binom{2n}{n} \frac{1}{n+1}  (z)^{n}                      \\
    \end{align}\pn
    
    Which is what we were looking for.
\end{proof}